Reduce F64

test/Test_GPU_HReduceF64Plus.cu
@@ -1,0 +1,31 @@
+#include <stdio.h>
+#include <stdint.h>
+#include "GPU_HReduceF64Plus.h"
+
+/* It would be nicer to write a purely-Pulse test. */
+int main()
+{
+	double *a;
+	double *ga;
+	const size_t siz = GPU_HReduceF64Plus_size;
+
+	a = (double*)malloc(siz * sizeof(double));
+	ga = (double*)PULSE_GPU_ALLOC(siz * sizeof(double));
+
+	int i;
+
+	for (i = 0; i < siz; i++)
+		a[i] = i;
+
+	MUST(cudaMemcpy(ga, a, siz * sizeof(double), cudaMemcpyHostToDevice));
+
+	PULSE_KCALL(GPU_HReduceF64Plus_k_reduce, 1, siz, siz, ga);
+
+	MUST(cudaMemcpy(a, ga, siz * sizeof(double), cudaMemcpyDeviceToHost));
+	MUST(cudaFree(ga));
+
+	printf("%lf\n", a[0]);
+	free(a);
+
+	return 0;
+}
