src/lib/GPU.Float64.fsti
@@ -14,3 +14,5 @@ let double = t
 [@@noextract_to "krml"] val mul : t -> t -> t
 [@@noextract_to "krml"] val div : t -> t -> t
 [@@noextract_to "krml"] val rem : t -> t -> t
+
+val add_comm (x y : t) : Lemma (add x y == add y x) [SMTPat (add x y)]
